Quasi-Internal Frame
====================

.. _fig-qiframe:
.. figure:: ../fig/qiframe.*
   :width: 300 px
   :align: center

   Global frame *g* and QI frame *i* of atoms 1 and 2.
   The z direction of this QI frame is chosen along the distance vector.

Rotation Matrix
---------------

Consider two vectors *u*, *v* and two reference frames *A*, *B*.
*R* is the rotation matrix of the *axes* such that

.. math::

   R u_A = u_B,

   R v_A = v_B.

Since :math:`u_A^T v_A=u_B^T v_B`,

.. math::

   R^T R=I.

A 2-D tensor, e.g., quadrupole moment *Q*, in two reference frames are
associated by

.. math::

   u_A^T Q_A v_A = u_B^T Q_B v_B.

It is easy to prove that

.. math::

   R Q_A R^T = Q_B.

Two common transformations used in Tinker are:

- From (A) *Local Frame* (in which parameters are provided)
  to (B) *Global Frame* (in which the calculation is done);
- From (A) *Global Frame* (for direct pairwise electrostatics)
  to (B) *Quasi-Internal (QI) Frame* (for optimized algebra),
  as shown in :numref:`fig-qiframe`.

Multipole Interaction in QI Frame
---------------------------------

Once the distance vector is in QI frame, many derivatives can be simplified
as shown in the following table. *f(r)* does not explicitly depend on
:math:`r_x,r_y,r_z`.

==================================  ==================  =============
Gradients                           Global Frame        QI Frame
==================================  ==================  =============
:math:`\partial f(r)/\partial x_2`  :math:`f'(r)r_x/r`  0
:math:`\partial f(r)/\partial y_2`  :math:`f'(r)r_y/r`  0
:math:`\partial f(r)/\partial z_2`  :math:`f'(r)r_z/r`  :math:`f'(r)`
==================================  ==================  =============

For potential energy, :eq:`pot4` can be used without modification in QI frame.
Since :math:`\partial\phi_1/\partial z_1 = -E_{z1}`, the z direction gradient
can be obtained from z direction electrostatic field (*Ez*):

.. math::

   \frac{\partial U}{\partial z}=-E_z C -E'_z D -E''_z Q -\cdots.

Once the torques are computed the same way as in the previous section

.. math::

   \tau = \tau_1 + \tau_2 = \boldsymbol{r}\times\boldsymbol{F}
        = (U'_x,U'_y,U'_z)\times(0,0,r) = (U'_y r, -U'_x r, 0),

x and y direction gradients then become

.. math::

   U'_x &= -\tau_y/r, \\
   U'_y &= \tau_x/r.

Depending on the direction of distance vector, the signs of x and y direction
gradients may flip.

Details
-------

In the following notes, :math:`A : B` stands for :math:`A = A + B`.
If there is no ambiguity, :math:`f'` and :math:`f''` may stand for
:math:`(f'_x,f'_y,f'_z)` and
:math:`(f''_{xx},f''_{yy},f''_{zz},f''_{xy},f''_{xz},f''_{yz})`, respectively.

================================  =================================================
Potential Terms                   Notes
================================  =================================================
:math:`\phi_1`                    :math:`\phi_1`
:math:`\phi'_{1x}`                :math:`\partial\phi_1/\partial x_1`
:math:`\phi'_{1y}`                :math:`\partial\phi_1/\partial y_1`
:math:`\phi'_{1z}`                :math:`\partial\phi_1/\partial z_1`
:math:`\phi''_{1xx}`              :math:`\partial^2\phi_1/\partial x_1^2`
:math:`\phi''_{1yy}`              :math:`\partial^2\phi_1/\partial y_1^2`
:math:`\phi''_{1zz}`              :math:`\partial^2\phi_1/\partial z_1^2`
:math:`\phi''_{1xy}`              :math:`\partial^2\phi_1/\partial x_1\partial y_1`
:math:`\phi''_{1xz}`              :math:`\partial^2\phi_1/\partial x_1\partial z_1`
:math:`\phi''_{1yz}`              :math:`\partial^2\phi_1/\partial y_1\partial z_1`
:math:`\phi_2`                    :math:`\phi_2`
:math:`\phi'_{2x}`                :math:`\partial\phi_2/\partial x_2`
:math:`\phi'_{2y}`                :math:`\partial\phi_2/\partial y_2`
:math:`\phi'_{2z}`                :math:`\partial\phi_2/\partial z_2`
:math:`\phi''_{2xx}`              :math:`\partial^2\phi_2/\partial x_2^2`
:math:`\phi''_{2yy}`              :math:`\partial^2\phi_2/\partial y_2^2`
:math:`\phi''_{2zz}`              :math:`\partial^2\phi_2/\partial z_2^2`
:math:`\phi''_{2xy}`              :math:`\partial^2\phi_2/\partial x_2\partial y_2`
:math:`\phi''_{2xz}`              :math:`\partial^2\phi_2/\partial x_2\partial z_2`
:math:`\phi''_{2yz}`              :math:`\partial^2\phi_2/\partial y_2\partial z_2`
================================  =================================================

Charge Terms
~~~~~~~~~~~~

.. math::

   \phi_1 &: T_{12}^{(1,1)} C_2 = B_0 C_2,\ \phi'_1 : T_{12}^{(2:4,1)} C_2 = \begin{pmatrix}
      0 \\
      0 \\
      r B_1 C_2 \end{pmatrix}, \\
   \phi''_1 &: T_{12}^{(5:13,1)} C_2 = -\begin{pmatrix}
      B_1 C_2 \\
      B_1 C_2 \\
      (B_1 - r^2 B_2) C_2 \\
      0 \\
      0 \\
      0 \end{pmatrix}.

.. math::

   \phi_2 &: T_{21}^{(1,1)} C_1 = B_0 C_1,\ \phi'_2 : T_{21}^{(2:4,1)} C_1 = -\begin{pmatrix}
      0 \\
      0 \\
      r B_1 C_1 \end{pmatrix}, \\
   \phi''_2 &: T_{21}^{(5:13,1)} C_1 = -\begin{pmatrix}
      B_1 C_1 \\
      B_1 C_1 \\
      (B_1 - r^2 B_2) C_1 \\
      0 \\
      0 \\
      0 \end{pmatrix}.

.. math::

   -E_{z1} &: r B_1 C_2,\ -E'_{z1} : -\begin{pmatrix}
      0 \\
      0 \\
      B_1 - r^2 B_2 \end{pmatrix}, \\
   -E''_{z1} &: -\begin{pmatrix}
      r B_2 C_2               \\
      r B_2 C_2               \\
      (3 r B_2 - r^3 B_3) C_2 \\
      0                       \\
      0                       \\
      0 \end{pmatrix}.

Dipole Terms
~~~~~~~~~~~~

.. math::

   \phi_1 &: T_{12}^{(1,2:4)} D_2 = -r B_1 D_{z2},\ \phi'_1 : T_{12}^{(2:4,2:4)} D_2 = \begin{pmatrix}
      B_1 D_{x2} \\
      B_1 D_{y2} \\
      (B_1 - r^2 B_2) D_{z2} \end{pmatrix}, \\
   \phi''_1 &: T_{12}^{(5:13,2:4)} D_2 = \begin{pmatrix}
      r B_2 D_{z2}               \\
      r B_2 D_{z2}               \\
      (3 r B_2 - r^3 B_3) D_{z2} \\
      0                          \\
      2 r B_2 D_{x2}             \\
      2 r B_2 D_{y2} \end{pmatrix}.

.. math::

   \phi_2 &: T_{21}^{(1,2:4)} D_1 = r B_1 D_{z1},\ \phi'_2 : T_{21}^{(2:4,2:4)} D_1 = \begin{pmatrix}
      B_1 D_{x1} \\
      B_1 D_{y1} \\
      (B_1 - r^2 B_2) D_{z1} \end{pmatrix}, \\
   \phi''_2 &: T_{21}^{(5:13,2:4)} D_1 = -\begin{pmatrix}
      r B_2 D_{z1}               \\
      r B_2 D_{z1}               \\
      (3 r B_2 - r^3 B_3) D_{z1} \\
      0                          \\
      2 r B_2 D_{x1}             \\
      2 r B_2 D_{y1} \end{pmatrix}.

.. math::

   -E_{z1} &: (B_1 - r^2 B_2) D_{z2},\ -E'_{z1} : \begin{pmatrix}
      r B_2 D_{x2} \\
      r B_2 D_{y2} \\
      (3 r B_2 - r^3 B_3) D_{z2} \end{pmatrix}, \\
   -E''_{z1} &: -\begin{pmatrix}
      (B_2 - r^2 B_3) D_{z2}               \\
      (B_2 - r^2 B_3) D_{z2}               \\
      (3 B_2 - 6 r^2 B_3 + r^4 B_4) D_{z2} \\
      0                                    \\
      2 (B_2 - r^2 B_3) D_{x2}             \\
      2 (B_2 - r^2 B_3) D_{y2} \end{pmatrix}.

Quadrupole Terms
~~~~~~~~~~~~~~~~

.. math::

   \phi_1 &: T_{12}^{(1,5:13)} Q_2 = r^2 B_2 Q_{zz2},\ \phi'_1 : T_{12}^{(2:4,5:13)} Q_2 = -\begin{pmatrix}
      2 r B_2 Q_{xz2} \\
      2 r B_2 Q_{yz2} \\
      (2 r B_2 - r^3 B_3) Q_{zz2} \end{pmatrix}, \\
   \phi''_1 &: T_{12}^{(5:13,5:13)} Q_2 = \begin{pmatrix}
      2 B_2 Q_{xx2} - r^2 B_3 Q_{zz2}       \\
      2 B_2 Q_{yy2} - r^2 B_3 Q_{zz2}       \\
      (2 B_2 - 5 r^2 B_3 + r^4 B_4) Q_{zz2} \\
      4 B_2 Q_{xy2}                         \\
      4 (B_2 - r^2 B_3) Q_{xz2}             \\
      4 (B_2 - r^2 B_3) Q_{yz2} \end{pmatrix}.

.. math::

   \phi_2 &: T_{21}^{(1,5:13)} Q_1 = r^2 B_2 Q_{zz1},\ \phi'_2 : T_{21}^{(2:4,5:13)} Q_1 = \begin{pmatrix}
      2 r B_2 Q_{xz1} \\
      2 r B_2 Q_{yz1} \\
      (2 r B_2 - r^3 B_3) Q_{zz1} \end{pmatrix}, \\
   \phi''_2 &: T_{21}^{(5:13,5:13)} Q_1 = \begin{pmatrix}
      2 B_2 Q_{xx1} - r^2 B_3 Q_{zz1}       \\
      2 B_2 Q_{yy1} - r^2 B_3 Q_{zz1}       \\
      (2 B_2 - 5 r^2 B_3 + r^4 B_4) Q_{zz1} \\
      4 B_2 Q_{xy1}                         \\
      4 (B_2 - r^2 B_3) Q_{xz1}             \\
      4 (B_2 - r^2 B_3) Q_{yz1} \end{pmatrix}.

.. math::

   -E_{z1} &: -(2 r B_2 - r^3 B_3) Q_{zz2},\ -E'_{z1} : \begin{pmatrix}
      2 (B_2 - r^2 B_3) Q_{xz2} \\
      2 (B_2 - r^2 B_3) Q_{yz2} \\
      (2 B_2 - 5 r^2 B_3 + r^4 B_4) Q_{zz2} \end{pmatrix}, \\
   -E''_{z1} &: \begin{pmatrix}
      -2 r B_3 Q_{yy2} - r^3 B_4 Q_{zz2}       \\
      -2 r B_3 Q_{xx2} - r^3 B_4 Q_{zz2}       \\
      (12 r B_3 - 9 r^3 B_4 + r^5 B_5) Q_{zz2} \\
      4 r B_3 Q_{xy2}                          \\
      4 (3 r B_3 - r^3 B_4) Q_{xz2}            \\
      4 (3 r B_3 - r^3 B_4) Q_{yz2} \end{pmatrix}.
